optimising erasure function

pcuic/theories/PCUICElimination.v
@@ -4,7 +4,7 @@ From Coq Require Import Bool String List Program BinPos Compare_dec Omega.
 From MetaCoq.Template Require Import config utils monad_utils BasicAst AstUtils.
 From MetaCoq.PCUIC Require Import PCUICTyping PCUICAst PCUICAstUtils PCUICInduction
      PCUICWeakening PCUICSubstitution PCUICRetyping PCUICMetaTheory PCUICWcbvEval
-     PCUICSR PCUICClosed PCUICInversion PCUICGeneration.
+     PCUICSR PCUICClosed PCUICInversion PCUICGeneration PCUICSafeLemmata.
 
 Definition Is_proof `{cf : checker_flags} Σ Γ t := ∑ T u, Σ ;;; Γ |- t : T × Σ ;;; Γ |- T : tSort u × is_prop_sort u.
 
@@ -16,6 +16,26 @@ Proof.
   intros [] []. unfold declared_minductive in *.
   rewrite H in H1. inversion H1. subst. rewrite H2 in H0. inversion H0. eauto.
 Qed.
+
+Definition SingletonProp `{cf : checker_flags} (Σ : global_env_ext) (ind : inductive) :=
+  forall mdecl idecl,
+    declared_inductive (fst Σ) mdecl ind idecl ->
+    forall Γ args u n (Σ' : global_env_ext),
+      wf Σ' ->
+      PCUICWeakeningEnv.extends Σ Σ' ->
+      welltyped Σ' Γ (mkApps (tConstruct ind n u) args) ->
+      ∥Is_proof Σ' Γ (mkApps (tConstruct ind n u) args)∥ /\
+       #|ind_ctors idecl| <= 1 /\
+       squash (All (Is_proof Σ' Γ) (skipn (ind_npars mdecl) args)).
+
+Definition Computational `{cf : checker_flags} (Σ : global_env_ext) (ind : inductive) :=
+  forall mdecl idecl,
+    declared_inductive (fst Σ) mdecl ind idecl ->
+    forall Γ args u n (Σ' : global_env_ext),
+      wf Σ' ->
+      PCUICWeakeningEnv.extends Σ Σ' ->
+      welltyped Σ' Γ (mkApps (tConstruct ind n u) args) ->
+      Is_proof Σ' Γ (mkApps (tConstruct ind n u) args) -> False.
 
 Definition Informative`{cf : checker_flags} (Σ : global_env_ext) (ind : inductive) :=
   forall mdecl idecl,
@@ -48,7 +68,6 @@ Proof.
   - admit. (* no idea what to do for Set *)
   - reflexivity.
 Admitted.                       (* elim_restriction_works *)
-
 
 Lemma elim_restriction_works_kelim2 `{cf : checker_flags} (Σ : global_env_ext) ind mind idecl : wf Σ ->
   declared_inductive (fst Σ) mind ind idecl ->
