extraction/theories/ESubstitution.v
@@ -49,6 +49,30 @@ Proof.
   eauto.
 Qed.
 
+Lemma SingletonProp_extends:
+  forall (Σ : global_env_ext) (ind : inductive)
+    (mdecl : PCUICAst.mutual_inductive_body) (idecl : PCUICAst.one_inductive_body),
+
+    PCUICTyping.declared_inductive (fst Σ) mdecl ind idecl ->
+    forall (Σ' : global_env) (u0 : universe_instance),
+      wf Σ' ->
+      extends Σ Σ' ->
+      SingletonProp Σ ind -> SingletonProp (Σ', Σ.2) ind.
+Proof.
+Admitted.
+
+Lemma Computational_extends:
+  forall (Σ : global_env_ext) (ind : inductive)
+    (mdecl : PCUICAst.mutual_inductive_body) (idecl : PCUICAst.one_inductive_body),
+
+    PCUICTyping.declared_inductive (fst Σ) mdecl ind idecl ->
+    forall (Σ' : global_env) (u0 : universe_instance),
+      wf Σ' ->
+      extends Σ Σ' ->
+      Computational Σ ind -> Computational (Σ', Σ.2) ind.
+Proof.
+Admitted.
+
 Lemma Informative_extends:
   forall (Σ : global_env_ext) (ind : inductive)
     (mdecl : PCUICAst.mutual_inductive_body) (idecl : PCUICAst.one_inductive_body),
@@ -89,8 +113,13 @@ Proof.
         eapply All2_impl. exact X3.
         intros. destruct H as [? []].
         split; eauto. }
-
-    eapply Informative_extends; eauto.
+    eapply Computational_extends; eauto.
+  - econstructor. all:eauto.
+    eapply SingletonProp_extends; eauto.
+    eapply Is_type_extends; eauto.
+    inv X3. eapply X7; eauto.
+  - eapply erases_tCase_Empty; eauto.
+    eapply SingletonProp_extends; eauto.
   - econstructor. destruct isdecl. 2:eauto.
     eapply Informative_extends; eauto.
   - econstructor.
@@ -178,6 +207,19 @@ Proof.
       destruct H. destruct p0.
       cbn. destruct x, y; cbn in *; subst.
       split; eauto.
+  - rewrite lift_mkApps. 
+
+    Lemma map_repeat X Y (f : X -> Y) x n :
+      map f (repeat x n) = repeat (f x) n.
+    Proof.
+      induction n; cbn; congruence.
+    Qed.
+    rewrite map_repeat. cbn. econstructor.
+    + eauto.
+    + eauto.
+    + eauto.
+    + admit.
+    + admit.
   - assert (HT : Σ;;; Γ ,,, Γ' |- PCUICAst.tFix mfix n : (decl.(dtype))).
     econstructor; eauto. eapply All_local_env_impl. eassumption. intros.
     destruct T; cbn in *; firstorder.
@@ -211,7 +253,7 @@ Proof.
     rewrite <- plus_n_O.
     now rewrite (All2_length _ _ H4).
   - eauto.
-Qed.
+Admitted.
 
 Lemma erases_weakening (Σ : global_env_ext) (Γ Γ' : PCUICAst.context) (t T : PCUICAst.term) t' :
   wf Σ ->
@@ -386,6 +428,8 @@ Proof.
     (*   eapply H4 in H5_; eauto. *)
     (*   inv X3. destruct X6. *)
     (*   eapply e; eauto. *)
+    + admit.
+    + admit.
     + econstructor.
       eapply is_type_subst; eauto.
   - inv H1.
@@ -449,4 +493,4 @@ Proof.
     + econstructor.
       eapply is_type_subst; eauto.
   - eapply H; eauto.
-Qed.
+Admitted.
